{
  "nbformat": 4,
  "nbformat_minor": 0,
  "metadata": {
    "colab": {
      "provenance": []
    },
    "kernelspec": {
      "name": "python3",
      "display_name": "Python 3"
    },
    "language_info": {
      "name": "python"
    }
  },
  "cells": [
    {
      "cell_type": "markdown",
      "source": [
        "# **Taylor Series: Academic Notes**\n",
        "\n",
        "### **Definition**\n",
        "A Taylor series represents a function $f(x)$ as an infinite sum of terms calculated from the derivatives of $f(x)$ at a single point $x_0$:\n",
        "$$\n",
        "f(x) = f(x_0) + f'(x_0)(x - x_0) + \\frac{f''(x_0)}{2!}(x - x_0)^2 + \\frac{f^{(3)}(x_0)}{3!}(x - x_0)^3 + \\cdots\n",
        "$$\n",
        "\n",
        "In summation notation:\n",
        "$$\n",
        "f(x) = \\sum_{n=0}^\\infty \\frac{f^{(n)}(x_0)}{n!}(x - x_0)^n,\n",
        "$$\n",
        "where:\n",
        "- $f^{(n)}(x_0)$ is the $n$-th derivative of $f(x)$ evaluated at $x_0$,\n",
        "- $n!$ is the factorial of $n$.\n",
        "\n",
        "---\n",
        "\n",
        "### **Maclaurin Series**\n",
        "The Taylor series centered at $x_0 = 0$ is called a **Maclaurin series**:\n",
        "$$\n",
        "f(x) = f(0) + f'(0)x + \\frac{f''(0)}{2!}x^2 + \\frac{f^{(3)}(0)}{3!}x^3 + \\cdots\n",
        "$$\n",
        "Or:\n",
        "$$\n",
        "f(x) = \\sum_{n=0}^\\infty \\frac{f^{(n)}(0)}{n!}x^n.\n",
        "$$\n",
        "\n",
        "---\n",
        "\n",
        "### **Common Taylor Series Expansions**\n",
        "\n",
        "1. **Exponential Function $e^x$:**\n",
        "   $$\n",
        "   e^x = 1 + x + \\frac{x^2}{2!} + \\frac{x^3}{3!} + \\cdots = \\sum_{n=0}^\\infty \\frac{x^n}{n!}.\n",
        "   $$\n",
        "\n",
        "2. **Sine Function $\\sin(x)$:**\n",
        "   $$\n",
        "   \\sin(x) = x - \\frac{x^3}{3!} + \\frac{x^5}{5!} - \\frac{x^7}{7!} + \\cdots = \\sum_{n=0}^\\infty \\frac{(-1)^n}{(2n+1)!}x^{2n+1}.\n",
        "   $$\n",
        "\n",
        "3. **Cosine Function $\\cos(x)$:**\n",
        "   $$\n",
        "   \\cos(x) = 1 - \\frac{x^2}{2!} + \\frac{x^4}{4!} - \\frac{x^6}{6!} + \\cdots = \\sum_{n=0}^\\infty \\frac{(-1)^n}{(2n)!}x^{2n}.\n",
        "   $$\n",
        "\n",
        "4. **Natural Logarithm $\\ln(1+x)$:**\n",
        "   Around $x = 0$ and valid for $|x| < 1$:\n",
        "   $$\n",
        "   \\ln(1+x) = x - \\frac{x^2}{2} + \\frac{x^3}{3} - \\frac{x^4}{4} + \\cdots = \\sum_{n=1}^\\infty \\frac{(-1)^{n+1}}{n}x^n.\n",
        "   $$\n",
        "\n",
        "5. **Rational Function $\\frac{1}{1-x}$:**\n",
        "   Around $x = 0$ and valid for $|x| < 1$:\n",
        "   $$\n",
        "   \\frac{1}{1-x} = 1 + x + x^2 + x^3 + \\cdots = \\sum_{n=0}^\\infty x^n.\n",
        "   $$\n",
        "\n",
        "---\n",
        "\n",
        "### **General Formula for Taylor Series**\n",
        "The general term of a Taylor series is:\n",
        "$$\n",
        "\\text{General Term: } \\frac{f^{(n)}(x_0)}{n!}(x - x_0)^n.\n",
        "$$\n",
        "\n",
        "### **Steps to Derive a Taylor Series**\n",
        "1. Compute the derivatives $f'(x), f''(x), f^{(3)}(x), \\dots$.\n",
        "2. Evaluate the derivatives at the expansion point $x_0$: $f(x_0), f'(x_0), f''(x_0), \\dots$.\n",
        "3. Substitute into the Taylor series formula:\n",
        "   $$\n",
        "   f(x) = \\sum_{n=0}^\\infty \\frac{f^{(n)}(x_0)}{n!}(x - x_0)^n.\n",
        "   $$\n",
        "\n",
        "---\n",
        "\n",
        "### **Taylor Polynomial (Truncated Series)**\n",
        "A Taylor polynomial is a finite approximation of the Taylor series:\n",
        "$$\n",
        "P_n(x) = f(x_0) + f'(x_0)(x - x_0) + \\frac{f''(x_0)}{2!}(x - x_0)^2 + \\cdots + \\frac{f^{(n)}(x_0)}{n!}(x - x_0)^n.\n",
        "$$\n",
        "\n",
        "---\n",
        "\n",
        "### **Error Estimate (Remainder Term)**\n",
        "The error in approximating $f(x)$ by a Taylor polynomial is given by the remainder term:\n",
        "$$\n",
        "R_n(x) = \\frac{f^{(n+1)}(c)}{(n+1)!}(x - x_0)^{n+1},\n",
        "$$\n",
        "where \\(c\\) is some value between \\(x\\) and \\(x_0\\).\n",
        "\n",
        "---\n",
        "\n",
        "### **Applications of Taylor Series**\n",
        "1. **Approximation of Functions**:\n",
        "   Use low-degree Taylor polynomials to approximate functions for small intervals around $x_0$.\n",
        "2. **Error Estimation**:\n",
        "   Use the remainder term $R_n(x)$ to estimate the error in the approximation.\n",
        "3. **Integration and Differentiation**:\n",
        "   Taylor series can be integrated or differentiated term by term.\n",
        "\n",
        "---\n",
        "\n",
        "### **Important Observations**\n",
        "1. The convergence of a Taylor series depends on the function and the point $x_0$.\n",
        "2. For analytic functions, the Taylor series converges to the function for all values of $x$ within the radius of convergence."
      ],
      "metadata": {
        "id": "o7sE3UklM_to"
      }
    },
    {
      "cell_type": "markdown",
      "source": [
        "#Student Exercises\n",
        "\n",
        "Taylor Series\n",
        "\n",
        "1. Find the Taylor series and visualize obtained functions in Geogebra:\n",
        "   - $f(x) = \\cos(x)$ around $x = 0$ up to the 4th degree.\n",
        "   - $h(x) = 1/(1-x)$ around $x = 0$ up to the 4rd degree.\n",
        "   - $g(x) = \\sin(x)$ around $x = \\pi$ up to the 4rd degree.\n",
        "\n",
        "2. Find a tangent line $y = f'(x_0) (x-x_0) + f(x_0)$ to the function $f(x) = e^{\\sin(x)}$ at $x_0 = \\pi$. Hints for Geogebra visualization: define f(x), include slider s, define y = f'(s) (x-s) + f(s), and include point P(s, f(s)).\n"
      ],
      "metadata": {
        "id": "2txrl4vQOaeu"
      }
    },
    {
      "cell_type": "markdown",
      "source": [
        "#1st question solution\n",
        "\n",
        "---\n",
        "\n",
        "## **Question 1: Find the Taylor series and visualize the obtained functions**\n",
        "\n",
        "### **(a) $f(x) = \\cos(x)$ around $x = 0$ up to the 4th degree**\n",
        "\n",
        "1. **Taylor Series Formula:**\n",
        "   $$\n",
        "   f(x) = \\sum_{n=0}^\\infty \\frac{f^{(n)}(x_0)}{n!}(x - x_0)^n\n",
        "   $$\n",
        "\n",
        "2. **Step 1: Compute Derivatives of $cos(x)$:**\n",
        "   - $f(x) = \\cos(x)$\n",
        "   - $f'(x) = -\\sin(x)$\n",
        "   - $f''(x) = -\\cos(x)$\n",
        "   - $f^{(3)}(x) = \\sin(x)$\n",
        "   - $f^{(4)}(x) = \\cos(x)$\n",
        "\n",
        "3. **Step 2: Evaluate Derivatives at $x_0 = 0$:**\n",
        "   - $f(0) = \\cos(0) = 1$\n",
        "   - $f'(0) = -\\sin(0) = 0$\n",
        "   - $f''(0) = -\\cos(0) = -1$\n",
        "   - $f^{(3)}(0) = \\sin(0) = 0$\n",
        "   - $f^{(4)}(0) = \\cos(0) = 1$\n",
        "\n",
        "4. **Step 3: Write the Taylor Series (up to the 4th degree):**\n",
        "   $$\n",
        "   \\cos(x) \\approx 1 - \\frac{x^2}{2!} + \\frac{x^4}{4!}\n",
        "   $$\n",
        "   Substituting factorial values:\n",
        "   $$\n",
        "   \\cos(x) \\approx 1 - \\frac{x^2}{2} + \\frac{x^4}{24}.\n",
        "   $$\n",
        "\n",
        "---\n",
        "\n",
        "### **(b) $h(x) = \\frac{1}{1-x}$ around $x = 0$ up to the 4th degree**\n",
        "\n",
        "1. **Taylor Series Formula for Rational Function:**\n",
        "   $$\n",
        "   \\frac{1}{1-x} = \\sum_{n=0}^\\infty x^n, \\quad \\text{for } |x| < 1.\n",
        "   $$\n",
        "\n",
        "2. **Write the Terms (up to the 4th degree):**\n",
        "   $$\n",
        "   \\frac{1}{1-x} \\approx 1 + x + x^2 + x^3 + x^4.\n",
        "   $$\n",
        "\n",
        "---\n",
        "\n",
        "### **(c) $g(x) = \\sin(x)$ around $x = \\pi$ up to the 4th degree**\n",
        "\n",
        "1. **Shift $x$ by $\\pi$:**\n",
        "   Let $x' = x - \\pi$, so the expansion is centered at $x = \\pi$.\n",
        "\n",
        "2. **Taylor Series Formula:**\n",
        "   $$\n",
        "   f(x) = \\sum_{n=0}^\\infty \\frac{f^{(n)}(\\pi)}{n!}(x - \\pi)^n.\n",
        "   $$\n",
        "\n",
        "3. **Step 1: Compute Derivatives of \\(\\sin(x)\\):**\n",
        "   - $f(x) = \\sin(x)$\n",
        "   - $f'(x) = \\cos(x)$\n",
        "   - $f''(x) = -\\sin(x)$\n",
        "   - $f^{(3)}(x) = -\\cos(x)$\n",
        "   - $f^{(4)}(x) = \\sin(x)$\n",
        "\n",
        "4. **Step 2: Evaluate Derivatives at $x_0 = \\pi$:**\n",
        "   - $f(\\pi) = \\sin(\\pi) = 0$\n",
        "   - $f'(\\pi) = \\cos(\\pi) = -1$\n",
        "   - $f''(\\pi) = -\\sin(\\pi) = 0$\n",
        "   - $f^{(3)}(\\pi) = -\\cos(\\pi) = 1$\n",
        "   - $f^{(4)}(\\pi) = \\sin(\\pi) = 0$\n",
        "\n",
        "5. **Step 3: Write the Taylor Series (up to the 4th degree):**\n",
        "   $$\n",
        "   \\sin(x) \\approx (x - \\pi) - \\frac{(x - \\pi)^3}{3!}.\n",
        "   $$\n",
        "   Substituting factorial values:\n",
        "   $$\n",
        "   \\sin(x) \\approx (x - \\pi) - \\frac{(x - \\pi)^3}{6}.\n",
        "   $$\n",
        "\n",
        "---\n",
        "\n",
        "## **Question 2: Tangent Line to $f(x) = e^{\\sin(x)}$ at $x_0 = \\pi$**\n",
        "\n",
        "1. **Tangent Line Formula:**\n",
        "   $$\n",
        "   y = f'(x_0)(x - x_0) + f(x_0).\n",
        "   $$\n",
        "\n",
        "2. **Step 1: Compute $f(x_0)$:**\n",
        "   $$\n",
        "   f(x) = e^{\\sin(x)}, \\quad f(\\pi) = e^{\\sin(\\pi)} = e^0 = 1.\n",
        "   $$\n",
        "\n",
        "3. **Step 2: Compute $f'(x)$:**\n",
        "   Using the chain rule:\n",
        "   $$\n",
        "   f'(x) = e^{\\sin(x)} \\cdot \\cos(x).\n",
        "   $$\n",
        "   At $x_0 = \\pi$:\n",
        "   $$\n",
        "   f'(\\pi) = e^{\\sin(\\pi)} \\cdot \\cos(\\pi) = 1 \\cdot (-1) = -1.\n",
        "   $$\n",
        "\n",
        "4. **Step 3: Write the Tangent Line:**\n",
        "   Substituting into the tangent line formula:\n",
        "   $$\n",
        "   y = -1(x - \\pi) + 1.\n",
        "   $$\n",
        "   Simplify:\n",
        "   $$\n",
        "   y = -x + \\pi + 1.\n",
        "   $$\n",
        "\n",
        "---"
      ],
      "metadata": {
        "id": "qiYsXNoROjeX"
      }
    },
    {
      "cell_type": "markdown",
      "source": [
        "#Geogebra visualizations\n",
        "1st question:\n",
        "\n",
        "a: https://www.geogebra.org/calculator/aqmdnz6x\n",
        "\n",
        "b:https://www.geogebra.org/calculator/b7v5ss4m\n",
        "\n",
        "c:https://www.geogebra.org/calculator/saqtq9jq\n",
        "\n",
        "2nd question: https://www.geogebra.org/calculator/udzzpusu\n",
        "\n"
      ],
      "metadata": {
        "id": "UsXBBFbrRM2S"
      }
    }
  ]
}