{
  "nbformat": 4,
  "nbformat_minor": 0,
  "metadata": {
    "colab": {
      "provenance": []
    },
    "kernelspec": {
      "name": "python3",
      "display_name": "Python 3"
    },
    "language_info": {
      "name": "python"
    }
  },
  "cells": [
    {
      "cell_type": "markdown",
      "source": [
        "$$\n",
        "\\textbf{18. Functions}\n",
        "$$\n",
        "\n",
        "\\textbf{Task 1}  \n",
        "Draw in a single Geogebra notebook the following functions:  \n",
        "\\( f(x) = x^2 \\),  \n",
        "\\( g(x) = x \\),  \n",
        "\\( h(x) = \\frac{1}{x} \\),  \n",
        "\\( j(x) = \\sin(x) \\).  \n",
        "Find the value of all the above functions at \\( x = 2 \\).\n",
        "\n",
        "At \\( x = 2 \\), we have:\n",
        "\n",
        "For \\( f(x) = x^2 \\):\n",
        "$$\n",
        "f(2) = 2^2 = 4\n",
        "$$\n",
        "\n",
        "For \\( g(x) = x \\):\n",
        "$$\n",
        "g(2) = 2\n",
        "$$\n",
        "\n",
        "For \\( h(x) = \\frac{1}{x} \\):\n",
        "$$\n",
        "h(2) = \\frac{1}{2}\n",
        "$$\n",
        "\n",
        "For \\( j(x) = \\sin(x) \\):\n",
        "$$\n",
        "j(2) = \\sin(2) \\approx 0.909\n",
        "$$\n",
        "\n",
        "https://www.geogebra.org/graphing/dpardvdw\n",
        "\n",
        "---\n",
        "\n",
        "\\textbf{Task 2}  \n",
        "Let \\( f(x) = 3x - 1 \\) and \\( g(x) = x \\). Find:\n",
        "\n",
        "1. \\( f(g(x)) \\):\n",
        "$$\n",
        "f(g(x)) = f(x) = 3x - 1\n",
        "$$\n",
        "\n",
        "2. \\( g(f(x)) \\):\n",
        "$$\n",
        "g(f(x)) = g(3x - 1) = 3x - 1\n",
        "$$\n",
        "\n",
        "3. \\( f(f(x)) \\):\n",
        "$$\n",
        "f(f(x)) = f(3x - 1) = 3(3x - 1) - 1 = 9x - 4\n",
        "$$\n",
        "\n",
        "4. \\( g(g(x)) \\):\n",
        "$$\n",
        "g(g(x)) = g(x) = x\n",
        "$$\n",
        "https://www.geogebra.org/graphing/dpardvdw\n",
        "---\n",
        "\n",
        "\\textbf{Task 3}  \n",
        "Let \\( f(x) = e^x \\) and \\( g(x) = \\ln(x) \\). Check:\n",
        "\n",
        "1. \\( f(g(x)) \\):\n",
        "$$\n",
        "f(g(x)) = f(\\ln(x)) = e^{\\ln(x)} = x\n",
        "$$\n",
        "\n",
        "2. \\( g(f(x)) \\):\n",
        "$$\n",
        "g(f(x)) = g(e^x) = \\ln(e^x) = x\n",
        "$$\n",
        "\n",
        "What do you notice?  \n",
        "We notice that \\( f(g(x)) = x \\) and \\( g(f(x)) = x \\), showing that the exponential and natural logarithm functions are inverses of each other.\n",
        "\n",
        "https://www.geogebra.org/graphing/dpardvdw\n",
        "---\n",
        "\n",
        "\\textbf{Task 4}  \n",
        "We have the function \\( f = \\{(1,7), (2,9), (3,11)\\} \\). Give the inverse function \\( f^{-1} \\).\n",
        "\n",
        "The inverse function \\( f^{-1} \\) switches the roles of the inputs and outputs. Thus, the inverse function is:\n",
        "$$\n",
        "f^{-1} = \\{(7,1), (9,2), (11,3)\\}\n",
        "$$\n",
        "https://www.geogebra.org/graphing/dpardvdw\n",
        "---\n",
        "\n",
        "\\textbf{Task 5}  \n",
        "We have the function \\( f = \\{(1,7), (2,7), (3,11)\\} \\). Give the inverse function \\( f^{-1} \\).\n",
        "\n",
        "The inverse function \\( f^{-1} \\) is:\n",
        "$$\n",
        "f^{-1} = \\{(7,1), (11,3)\\}\n",
        "$$\n",
        "Note: \\( f(x) = 7 \\) has no unique inverse because it is not one-to-one.\n",
        "https://www.geogebra.org/graphing/dpardvdw\n",
        "---\n",
        "\n",
        "\\textbf{Task 6}  \n",
        "We have the function \\( f(x) = x - 1 \\). Give the inverse function \\( f^{-1} \\).\n",
        "\n",
        "To find the inverse function, we solve for \\( x \\) in terms of \\( y \\) from the equation \\( y = x - 1 \\):\n",
        "$$\n",
        "x = y + 1\n",
        "$$\n",
        "Thus, the inverse function is:\n",
        "$$\n",
        "f^{-1}(x) = x + 1\n",
        "$$\n",
        "\n",
        "Show both functions on the same Geogebra notebook.\n",
        "\n",
        "https://www.geogebra.org/graphing/dpardvdw"
      ],
      "metadata": {
        "id": "fB6WzljKv5-t"
      }
    },
    {
      "cell_type": "markdown",
      "source": [
        "$$\n",
        "\\textbf{19. Limits of Sequences}\n",
        "$$\n",
        "\n",
        "\\textbf{Task 1}  \n",
        "Calculate:  \n",
        "$$\n",
        "\\lim_{{n \\to \\infty}} \\frac{n^2 + 3n}{2n^2 - 2n}\n",
        "$$\n",
        "\n",
        "Simplifying the expression:\n",
        "$$\n",
        "\\frac{n^2 + 3n}{2n^2 - 2n} = \\frac{n^2(1 + \\frac{3}{n})}{n^2(2 - \\frac{2}{n})}\n",
        "$$\n",
        "As \\(n \\to \\infty\\), the terms involving \\( \\frac{1}{n} \\) approach zero, and the limit is:\n",
        "$$\n",
        "\\lim_{{n \\to \\infty}} \\frac{n^2(1 + \\frac{3}{n})}{n^2(2 - \\frac{2}{n})} = \\frac{1}{2}\n",
        "$$\n",
        "\n",
        "---\n",
        "\n",
        "\\textbf{Task 2}  \n",
        "Calculate:  \n",
        "$$\n",
        "\\lim_{{n \\to \\infty}} \\frac{(2n + 3)}{3n^3 - 1}\n",
        "$$\n",
        "\n",
        "As \\(n \\to \\infty\\), the highest degree terms dominate:\n",
        "$$\n",
        "\\lim_{{n \\to \\infty}} \\frac{2n + 3}{3n^3 - 1} = \\lim_{{n \\to \\infty}} \\frac{2n}{3n^3} = \\lim_{{n \\to \\infty}} \\frac{2}{3n^2} = 0\n",
        "$$\n",
        "\n",
        "---\n",
        "\n",
        "\\textbf{Task 3}  \n",
        "Prove using the squeeze theorem:  \n",
        "$$\n",
        "\\lim_{{n \\to \\infty}} \\frac{\\sin(n)}{n}\n",
        "$$\n",
        "\n",
        "We know that:\n",
        "$$\n",
        "-1 \\leq \\sin(n) \\leq 1\n",
        "$$\n",
        "Thus:\n",
        "$$\n",
        "\\frac{-1}{n} \\leq \\frac{\\sin(n)}{n} \\leq \\frac{1}{n}\n",
        "$$\n",
        "As \\( n \\to \\infty \\), both \\( \\frac{-1}{n} \\) and \\( \\frac{1}{n} \\) approach 0. Therefore, by the squeeze theorem:\n",
        "$$\n",
        "\\lim_{{n \\to \\infty}} \\frac{\\sin(n)}{n} = 0\n",
        "$$\n",
        "\n",
        "---\n",
        "\n",
        "\\textbf{Task 4}  \n",
        "Find the limit of the sequence:  \n",
        "$$\n",
        "a_n = \\left( 1 + \\frac{1}{n} \\right)^n\n",
        "$$\n",
        "\n",
        "This is a well-known limit:\n",
        "$$\n",
        "\\lim_{{n \\to \\infty}} \\left( 1 + \\frac{1}{n} \\right)^n = e\n",
        "$$\n",
        "\n",
        "---\n",
        "\n",
        "$$\n",
        "\\textbf{20. Limits of Real Functions}\n",
        "$$\n",
        "\n",
        "\\textbf{Task 1}  \n",
        "Compute:  \n",
        "$$\n",
        "\\lim_{{x \\to \\infty}} \\frac{x^3 + 2x^2}{x^4 - 3x^3}\n",
        "$$\n",
        "\n",
        "Dividing both the numerator and denominator by \\( x^4 \\):\n",
        "$$\n",
        "\\lim_{{x \\to \\infty}} \\frac{x^3 + 2x^2}{x^4 - 3x^3} = \\lim_{{x \\to \\infty}} \\frac{\\frac{x^3}{x^4} + \\frac{2x^2}{x^4}}{1 - \\frac{3x^3}{x^4}} = \\lim_{{x \\to \\infty}} \\frac{\\frac{1}{x} + \\frac{2}{x^2}}{1 - \\frac{3}{x}} = 0\n",
        "$$\n",
        "\n",
        "---\n",
        "\n",
        "\\textbf{Task 2}  \n",
        "Find:  \n",
        "$$\n",
        "\\lim_{{x \\to 0}} \\frac{\\sin(3x)}{2x + 1}\n",
        "$$\n",
        "\n",
        "Using the fact that \\( \\lim_{{x \\to 0}} \\sin(3x) = 3x \\), we have:\n",
        "$$\n",
        "\\lim_{{x \\to 0}} \\frac{\\sin(3x)}{2x + 1} = \\lim_{{x \\to 0}} \\frac{3x}{2x + 1} = \\frac{0}{1} = 0\n",
        "$$\n",
        "\n",
        "---\n",
        "\n",
        "\\textbf{Task 3}  \n",
        "Find the asymptotes of the function:  \n",
        "\n",
        "1. For \\( f(x) = \\frac{x^2 - 1}{x^2 + 1} \\), the horizontal asymptote is:\n",
        "$$\n",
        "\\lim_{{x \\to \\infty}} f(x) = \\lim_{{x \\to \\infty}} \\frac{x^2 - 1}{x^2 + 1} = \\frac{1 - 0}{1 + 0} = 1\n",
        "$$\n",
        "Thus, the horizontal asymptote is \\( y = 1 \\).\n",
        "\n",
        "2. For \\( g(x) = \\frac{\\sin(x)}{x^2 + 1} \\), the horizontal asymptote is:\n",
        "$$\n",
        "\\lim_{{x \\to \\infty}} g(x) = \\lim_{{x \\to \\infty}} \\frac{\\sin(x)}{x^2 + 1} = 0\n",
        "$$\n",
        "Thus, the horizontal asymptote is \\( y = 0 \\).\n"
      ],
      "metadata": {
        "id": "8pCxgY3Yv8uO"
      }
    }
  ]
}